src/FCF/FCF.v
@@ -3,3 +3,5 @@ Require Export ProgramLogic.
 Require Export ProgTacs.
 Require Export RndNat.
 Require Export GenTacs.
+
+Open Scope eq_scope.
