README.md
@@ -1,2 +1,10 @@
 # fcf
 Foundational Cryptography Framework for machine-checked proofs of cryptography.  
+
+Getting Started:
+1) cd FCF
+
+2) make
+
+Then open a simple example from the “examples” directory in Proof General.  A good place to start is “ElGamal.v.”  Interactively step through this proof to learn how a 
+
